ModularEngine/src/LogicEngine.FStar/subst.fst
@@ -1,13 +1,12 @@
 module Subst
-open TypeHeaders
 open Types
 open Util
 
-extern reference Utilities {
-    language="F#";
-    dll="LogicEngine.FStar";
-    namespace="Microsoft.Research.Dkal.LogicEngine.FStar";
-    classname="Utilities"}
+
+val subst_apply : substitution -> var -> term
+let subst_apply s v = match assoc v s with 
+  | None -> Var v
+  | Some t -> t
 
 (* Axiomatization of sets of variables *)
 logic function Empty : vars
@@ -23,12 +22,14 @@ logic function Select : substitution -> var -> term
 logic function Update : substitution -> var -> term -> substitution
 assume forall (s:substitution) (x:var) (t:term). (Select (Update s x t) x) = t
 assume forall (s:substitution) (x:var) (y:var) (t:term). (x <> y) => ((Select (Update s x t) y) = (Select s y))
+assume forall (s:substitution) (x:var) (t:term). (Update s x t) = ((x,t)::s)
 
 (* Domain of a substitution will be restricted to be a subset of the unification variables *)
 logic function Domain : substitution -> vars
 logic function EmptySubst : substitution
 assume forall (s:substitution) (x:var) (t:term). Domain (Update s x t) = (Union (Domain s) (Singleton x))
 assume (Domain EmptySubst) = Empty
+assume (EmptySubst = []) 
 
 (* freevars of both the domain and the range *)
 (* the set of variables is represented as a list with possible double occurrences
@@ -82,15 +83,11 @@ assume (MkSubst [] [] = EmptySubst)
 assume (forall (x:var) (t:term) (xs:vars) (ts:list term). (MkSubst (x::xs) (t::ts)) = (Update (MkSubst xs ts) x t))
 (* solution 1 (preferred but the F# file does not compile, see utilities.fs) *)
 
-extern Utilities val mkSubst : xs:vars -> ts:list term -> s:substitution{s=(MkSubst xs ts)}
-
-(* solution 2 (but it does not allow to put any arbitrary output refinement) *)
-(*
-extern Utilities val mkSubst_aux : xs:listFS var -> ts:listFS term -> substitution
-val mkSubst : xs:vars -> ts:list term -> substitution
-let mkSubst xs ts =
-  mkSubst_aux (ListOfPrimsList xs) (ListOfPrimsList ts)
-*)
+val mkSubst: xs:vars -> ts:list term -> s:substitution{s=(MkSubst xs ts)}
+let mkSubst xs ts = 
+  let s = zip xs ts in 
+    assume (s=(MkSubst xs ts));
+    s
 
 type Extends :: substitution => substitution => E
 assume forall (s:substitution). Extends s s
@@ -99,43 +96,59 @@ assume forall (s1:substitution) (s2:substitution) (x:var) (t:term).
         => Extends (Update s2 x t) s1
 (* what if x appears free in some elements of the image of s2?? *)
 
-extern Utilities val substQuery: q:ISubstrateQueryTerm -> s:substitution -> q':ISubstrateQueryTerm{(SubstQuery q s)=q'}
-extern Utilities val emptySubst: bool -> s:substitution{s=EmptySubst}
+val substQuery: q:ISubstrateQueryTerm -> s:substitution -> q':ISubstrateQueryTerm{(SubstQuery q s)=q'}
+
+val emptySubst: unit -> s:substitution{s=EmptySubst}
+let emptySubst b = []
+ 
 
 (* TODO: dummy, need to get rid of it eventually *)
-extern Utilities val extends : 
-     s2:substitution
-  -> s1:substitution 
-  -> b:bool{((b=true) <=> (Extends s2 s1))}
+val extends : s2:substitution
+           -> s1:substitution 
+           -> b:bool{((b=true) <=> (Extends s2 s1))}
+let extends s2 s1 = raise "NYI"
 
-extern Utilities val lookupVar : 
-     s:substitution 
-  -> x:var 
-  -> o:option term{((o=None <=> (not (In x (Domain s)))) &&
-                      (forall (t:term). (o=(Some t)) => 
-   			  ((In x (Domain s)) && (t=(Select s x)))))} 
+type PostLookup :: _ = (fun (s:substitution) (x:var) (o:option term) =>
+    ((o=None <=> (not (In x (Domain s)))) &&
+                      (forall (t:term). (o=(Some t)) =>
+   			  ((In x (Domain s)) && (t=(Select s x))))))
+val lookupVar :
+     s:substitution
+  -> x:var
+  -> o:option term{PostLookup s x o}
+let lookupVar s x =
+  let o = assoc x s in
+    assume (PostLookup s x o);
+    o
 
-extern Utilities val extendSubst : 
-     s:substitution 
-  -> x:var 
+val extendSubst :
+     s:substitution
+  -> x:var
   -> t:term(*{(Subst t s)=t && not(In x (Domain s))}*) (* TODO *)
   -> s':substitution{s'=(Update s x t)}
+let extendSubst s x t = (x,t)::s
 
-extern Utilities val domain : s:substitution -> v:vars{(v = (Domain s))}
+val domain : s:substitution -> v:vars{(v = (Domain s))}
+let domain s =
+  let v = map (fun (x,_) -> x)  s in
+    assume (v=(Domain s));
+    v
 
-val inDomain : 
-     s:substitution 
-  -> x:var 
+val inDomain :
+     s:substitution
+  -> x:var
   -> b:bool{b=true <=> In x (Domain s)}
 let inDomain s x =
   contains x (domain s)
 
-extern Utilities val substrateQueryTerm_Vars :
+val substrateQueryTerm_Vars :
   s:ISubstrateQueryTerm -> f:vars{(f = (FreeVars (SubstrateQueryTerm s)))}
-extern Utilities val substrateUpdateTerm_Vars :
+
+val substrateUpdateTerm_Vars :
   s:ISubstrateUpdateTerm -> f:vars{(f = (FreeVars (SubstrateUpdateTerm s)))}
-val freeVars : 
-     t:term 
+
+val freeVars :
+     t:term
   -> f:vars{(f = (FreeVars t))}
 let rec freeVars t = match t with
   | Var x -> [x]
@@ -154,28 +167,22 @@ let rec freeVarsSubst_aux s v =
              | None -> failwith "impos"
 			 | Some(t) -> append (freeVars t) (freeVarsSubst_aux s tl))
 
-val freeVarsSubst : (* maybe a way to not make it extern? *) 
-     s:substitution 
+val freeVarsSubst : (* maybe a way to not make it extern? *)
+     s:substitution
   -> f:vars{(f = (FreeVarsSubst s))}
-let freeVarsSubst s =
-  freeVarsSubst_aux s (domain s)
-(* collect (fun k -> match lookupVar s k with
-                    | None -> [ ]
-					| Some(t) -> freeVars t
-		  ) (domain s) *)
+let freeVarsSubst s = freeVarsSubst_aux s (domain s)
     
-val inFreevars : 
-     s:substitution 
-  -> x:var 
+val inFreevars :
+     s:substitution
+  -> x:var
   -> b:bool{b=true <=> In x (FreeVarsSubst s)}
 let inFreevars s x =
   contains x (freeVarsSubst s)
 
-
 let genId =
-  let ctr = ref 0 in 
-    fun (x:unit) -> 
-      (ctr := !ctr + 1); 
+  let ctr = newref 0 in
+    fun (x:unit) ->
+      (ctr := !ctr + 1);
       !ctr
 
 val freshVar : ty:typ -> x:var{x.typ=ty}
@@ -184,21 +191,21 @@ let freshVar ty = { typ = ty; name = (Concat "__fresh" (string_of_any (genId()))
 type varTyEq :: _ = (fun (x:var) (y:var) => (x.typ=y.typ))
 type varsTyEq :: _ = (fun (xs:vars) (ys:vars) => (ZipE var var varTyEq xs ys))
 val freshVars: xs:vars -> (ys:vars * varsTyEq xs ys)
-let rec freshVars xs = match xs with 
+let rec freshVars xs = match xs with
   | [] -> ([], ZipE_Nil<var, var, varTyEq>)
-  | x::xtl -> 
-      let y = freshVar x.typ in 
-      let ytl, ztl = freshVars xtl in 
+  | x::xtl ->
+      let y = freshVar x.typ in
+      let ytl, ztl = freshVars xtl in
         ((y::ytl), ZipE_Cons<var,var,varTyEq> xtl ytl x y ztl)
 
   
 (* see term_apply in term.fst *)
-(* NS: Would be nice to have this be the only definition of subst 
+(* NS: Would be nice to have this be the only definition of subst
        and generate the logic function axioms from this code. *)
 val subst: i:term -> s:substitution -> i':term{(Subst i s)=i'}
 val substList : tl:list term -> s:substitution -> tl':list term{(SubstList tl s)=tl'}
 let rec subst i s = match i with
-  | Var y -> (match lookupVar s y with 
+  | Var y -> (match lookupVar s y with
                 | None -> Var y
                 | Some t -> t)
   | Const c -> Const c
@@ -208,8 +215,8 @@ let rec subst i s = match i with
 	
 and substList ilist s = match ilist with
   | [] -> []
-  | hd::tl -> 
-      let tl' = substList tl s in 
+  | hd::tl ->
+      let tl' = substList tl s in
       let hd' = subst hd s in
-        Cons<term> hd' tl' (* type inference is too eager here and infers a refined instantiation; 
+        Cons<term> hd' tl' (* type inference is too eager here and infers a refined instantiation;
                               need to provide explicit annotation on Cons *)
